<?xml version="1.0"?>


<!DOCTYPE rdf:RDF [
    <!ENTITY owl "http://www.w3.org/2002/07/owl#" >
    <!ENTITY xsd "http://www.w3.org/2001/XMLSchema#" >
    <!ENTITY rdfs "http://www.w3.org/2000/01/rdf-schema#" >
    <!ENTITY rdf "http://www.w3.org/1999/02/22-rdf-syntax-ns#" >
]>


<rdf:RDF xmlns="http://www.w3.org/2002/07/owl#"
     xml:base="http://www.w3.org/2002/07/owl"
     xmlns:rdfs="http://www.w3.org/2000/01/rdf-schema#"
     xmlns:owl="http://www.w3.org/2002/07/owl#"
     xmlns:xsd="http://www.w3.org/2001/XMLSchema#"
     xmlns:rdf="http://www.w3.org/1999/02/22-rdf-syntax-ns#">
    <Ontology rdf:about="http://www.agilebirds.com/ontologies/CostaBusinessArchitecture.owl"/>
    


    <!-- 
    ///////////////////////////////////////////////////////////////////////////////////////
    //
    // Object Properties
    //
    ///////////////////////////////////////////////////////////////////////////////////////
     -->

    


    <!-- http://www.agilebirds.com/ontologies/CostaBusinessArchitecture.owl#Type -->

    <ObjectProperty rdf:about="http://www.agilebirds.com/ontologies/CostaBusinessArchitecture.owl#Type">
        <rdfs:comment>
An optional association that specifies the link corresponding to this connector.

&quot;A type is a named element that is used as the type for a typed element. 
A type constrains the values represented by a typed element.&quot;</rdfs:comment>
        <rdfs:comment>This information is derived from the return result for this Operation.
The type of the TypedElement.</rdfs:comment>
        <rdfs:range rdf:resource="http://www.agilebirds.com/ontologies/CostaBusinessArchitecture.owl#Association"/>
        <rdfs:range rdf:resource="http://www.agilebirds.com/ontologies/CostaBusinessArchitecture.owl#Type"/>
        <rdfs:domain rdf:resource="http://www.agilebirds.com/ontologies/CostaBusinessArchitecture.owl#TypedElement"/>
    </ObjectProperty>
    


    <!-- http://www.agilebirds.com/ontologies/CostaBusinessArchitecture.owl#hasActivity -->

    <ObjectProperty rdf:about="http://www.agilebirds.com/ontologies/CostaBusinessArchitecture.owl#hasActivity">
        <rdfs:domain rdf:resource="http://www.agilebirds.com/ontologies/CostaBusinessArchitecture.owl#ValueStream"/>
        <rdfs:range rdf:resource="http://www.agilebirds.com/ontologies/CostaBusinessArchitecture.owl#ValueStreamActivity"/>
        <rdfs:subPropertyOf rdf:resource="&owl;topObjectProperty"/>
    </ObjectProperty>
    


    <!-- http://www.agilebirds.com/ontologies/CostaBusinessArchitecture.owl#hasCapability -->

    <ObjectProperty rdf:about="http://www.agilebirds.com/ontologies/CostaBusinessArchitecture.owl#hasCapability">
        <rdfs:range rdf:resource="http://www.agilebirds.com/ontologies/CostaBusinessArchitecture.owl#Capability"/>
        <rdfs:domain rdf:resource="http://www.agilebirds.com/ontologies/CostaBusinessArchitecture.owl#CapacityContrainer"/>
    </ObjectProperty>
    


    <!-- http://www.agilebirds.com/ontologies/CostaBusinessArchitecture.owl#hasDiagram -->

    <ObjectProperty rdf:about="http://www.agilebirds.com/ontologies/CostaBusinessArchitecture.owl#hasDiagram">
        <rdfs:domain rdf:resource="http://www.agilebirds.com/ontologies/CostaBusinessArchitecture.owl#NamedElement"/>
        <rdfs:range rdf:resource="http://www.agilebirds.com/ontologies/CostaBusinessArchitecture.owl#View"/>
    </ObjectProperty>
    


    <!-- http://www.agilebirds.com/ontologies/CostaBusinessArchitecture.owl#hasGoal -->

    <ObjectProperty rdf:about="http://www.agilebirds.com/ontologies/CostaBusinessArchitecture.owl#hasGoal">
        <rdfs:range rdf:resource="http://www.agilebirds.com/ontologies/CostaBusinessArchitecture.owl#Goal"/>
        <rdfs:domain rdf:resource="http://www.agilebirds.com/ontologies/CostaBusinessArchitecture.owl#ProductSegmentation"/>
        <rdfs:domain rdf:resource="http://www.agilebirds.com/ontologies/CostaBusinessArchitecture.owl#ServiceBreakdown"/>
        <rdfs:subPropertyOf rdf:resource="&owl;topObjectProperty"/>
    </ObjectProperty>
    


    <!-- http://www.agilebirds.com/ontologies/CostaBusinessArchitecture.owl#hasHotMapValue -->

    <ObjectProperty rdf:about="http://www.agilebirds.com/ontologies/CostaBusinessArchitecture.owl#hasHotMapValue">
        <rdfs:domain rdf:resource="http://www.agilebirds.com/ontologies/CostaBusinessArchitecture.owl#CostaElement"/>
        <rdfs:range rdf:resource="http://www.agilebirds.com/ontologies/CostaBusinessArchitecture.owl#HotMapValue"/>
    </ObjectProperty>
    


    <!-- http://www.agilebirds.com/ontologies/CostaBusinessArchitecture.owl#hasProductSegmentation -->

    <ObjectProperty rdf:about="http://www.agilebirds.com/ontologies/CostaBusinessArchitecture.owl#hasProductSegmentation">
        <rdfs:range rdf:resource="http://www.agilebirds.com/ontologies/CostaBusinessArchitecture.owl#ProductSegmentation"/>
        <rdfs:subPropertyOf rdf:resource="&owl;topObjectProperty"/>
        <rdfs:domain>
            <Class>
                <unionOf rdf:parseType="Collection">
                    <rdf:Description rdf:about="http://www.agilebirds.com/ontologies/CostaBusinessArchitecture.owl#Goal"/>
                    <rdf:Description rdf:about="http://www.agilebirds.com/ontologies/CostaBusinessArchitecture.owl#ProductSegmentationContainer"/>
                </unionOf>
            </Class>
        </rdfs:domain>
    </ObjectProperty>
    


    <!-- http://www.agilebirds.com/ontologies/CostaBusinessArchitecture.owl#hasServiceBreakdown -->

    <ObjectProperty rdf:about="http://www.agilebirds.com/ontologies/CostaBusinessArchitecture.owl#hasServiceBreakdown">
        <rdfs:range rdf:resource="http://www.agilebirds.com/ontologies/CostaBusinessArchitecture.owl#ServiceBreakdown"/>
        <rdfs:domain>
            <Class>
                <unionOf rdf:parseType="Collection">
                    <rdf:Description rdf:about="http://www.agilebirds.com/ontologies/CostaBusinessArchitecture.owl#Goal"/>
                    <rdf:Description rdf:about="http://www.agilebirds.com/ontologies/CostaBusinessArchitecture.owl#ServiceBreakdownContainer"/>
                </unionOf>
            </Class>
        </rdfs:domain>
    </ObjectProperty>
    


    <!-- http://www.agilebirds.com/ontologies/CostaBusinessArchitecture.owl#hasValueStream -->

    <ObjectProperty rdf:about="http://www.agilebirds.com/ontologies/CostaBusinessArchitecture.owl#hasValueStream">
        <rdfs:domain rdf:resource="http://www.agilebirds.com/ontologies/CostaBusinessArchitecture.owl#Goal"/>
        <rdfs:range rdf:resource="http://www.agilebirds.com/ontologies/CostaBusinessArchitecture.owl#ValueStream"/>
        <inverseOf rdf:resource="http://www.agilebirds.com/ontologies/CostaBusinessArchitecture.owl#isValueStreamOf"/>
    </ObjectProperty>
    


    <!-- http://www.agilebirds.com/ontologies/CostaBusinessArchitecture.owl#isActivityOf -->

    <ObjectProperty rdf:about="http://www.agilebirds.com/ontologies/CostaBusinessArchitecture.owl#isActivityOf">
        <rdfs:range rdf:resource="http://www.agilebirds.com/ontologies/CostaBusinessArchitecture.owl#ValueStream"/>
        <rdfs:domain rdf:resource="http://www.agilebirds.com/ontologies/CostaBusinessArchitecture.owl#ValueStreamActivity"/>
        <inverseOf rdf:resource="http://www.agilebirds.com/ontologies/CostaBusinessArchitecture.owl#hasActivity"/>
    </ObjectProperty>
    


    <!-- http://www.agilebirds.com/ontologies/CostaBusinessArchitecture.owl#isCapabilityOf -->

    <ObjectProperty rdf:about="http://www.agilebirds.com/ontologies/CostaBusinessArchitecture.owl#isCapabilityOf">
        <rdfs:domain rdf:resource="http://www.agilebirds.com/ontologies/CostaBusinessArchitecture.owl#Capability"/>
        <rdfs:range rdf:resource="http://www.agilebirds.com/ontologies/CostaBusinessArchitecture.owl#CapacityContrainer"/>
        <inverseOf rdf:resource="http://www.agilebirds.com/ontologies/CostaBusinessArchitecture.owl#hasCapability"/>
    </ObjectProperty>
    


    <!-- http://www.agilebirds.com/ontologies/CostaBusinessArchitecture.owl#isCapabilityOfActivity -->

    <ObjectProperty rdf:about="http://www.agilebirds.com/ontologies/CostaBusinessArchitecture.owl#isCapabilityOfActivity">
        <rdfs:domain rdf:resource="http://www.agilebirds.com/ontologies/CostaBusinessArchitecture.owl#Capability"/>
        <rdfs:range rdf:resource="http://www.agilebirds.com/ontologies/CostaBusinessArchitecture.owl#ValueStreamActivity"/>
    </ObjectProperty>
    


    <!-- http://www.agilebirds.com/ontologies/CostaBusinessArchitecture.owl#isGoalOf -->

    <ObjectProperty rdf:about="http://www.agilebirds.com/ontologies/CostaBusinessArchitecture.owl#isGoalOf">
        <rdfs:domain rdf:resource="http://www.agilebirds.com/ontologies/CostaBusinessArchitecture.owl#Goal"/>
        <rdfs:range rdf:resource="http://www.agilebirds.com/ontologies/CostaBusinessArchitecture.owl#ProductSegmentation"/>
        <rdfs:range rdf:resource="http://www.agilebirds.com/ontologies/CostaBusinessArchitecture.owl#ServiceBreakdown"/>
        <inverseOf rdf:resource="http://www.agilebirds.com/ontologies/CostaBusinessArchitecture.owl#hasGoal"/>
        <rdfs:subPropertyOf rdf:resource="&owl;topObjectProperty"/>
    </ObjectProperty>
    


    <!-- http://www.agilebirds.com/ontologies/CostaBusinessArchitecture.owl#isProductSegmentationOf -->

    <ObjectProperty rdf:about="http://www.agilebirds.com/ontologies/CostaBusinessArchitecture.owl#isProductSegmentationOf">
        <rdfs:domain rdf:resource="http://www.agilebirds.com/ontologies/CostaBusinessArchitecture.owl#ProductSegmentation"/>
        <inverseOf rdf:resource="http://www.agilebirds.com/ontologies/CostaBusinessArchitecture.owl#hasProductSegmentation"/>
        <rdfs:range>
            <Class>
                <unionOf rdf:parseType="Collection">
                    <rdf:Description rdf:about="http://www.agilebirds.com/ontologies/CostaBusinessArchitecture.owl#Goal"/>
                    <rdf:Description rdf:about="http://www.agilebirds.com/ontologies/CostaBusinessArchitecture.owl#ProductSegmentationContainer"/>
                </unionOf>
            </Class>
        </rdfs:range>
    </ObjectProperty>
    


    <!-- http://www.agilebirds.com/ontologies/CostaBusinessArchitecture.owl#isServiceBreakdownOf -->

    <ObjectProperty rdf:about="http://www.agilebirds.com/ontologies/CostaBusinessArchitecture.owl#isServiceBreakdownOf">
        <rdfs:domain rdf:resource="http://www.agilebirds.com/ontologies/CostaBusinessArchitecture.owl#ServiceBreakdown"/>
        <inverseOf rdf:resource="http://www.agilebirds.com/ontologies/CostaBusinessArchitecture.owl#hasServiceBreakdown"/>
        <rdfs:range>
            <Class>
                <unionOf rdf:parseType="Collection">
                    <rdf:Description rdf:about="http://www.agilebirds.com/ontologies/CostaBusinessArchitecture.owl#Goal"/>
                    <rdf:Description rdf:about="http://www.agilebirds.com/ontologies/CostaBusinessArchitecture.owl#ServiceBreakdownContainer"/>
                </unionOf>
            </Class>
        </rdfs:range>
    </ObjectProperty>
    


    <!-- http://www.agilebirds.com/ontologies/CostaBusinessArchitecture.owl#isValueStreamOf -->

    <ObjectProperty rdf:about="http://www.agilebirds.com/ontologies/CostaBusinessArchitecture.owl#isValueStreamOf">
        <rdfs:range rdf:resource="http://www.agilebirds.com/ontologies/CostaBusinessArchitecture.owl#Goal"/>
        <rdfs:domain rdf:resource="http://www.agilebirds.com/ontologies/CostaBusinessArchitecture.owl#ValueStream"/>
    </ObjectProperty>
    


    <!-- http://www.agilebirds.com/ontologies/CostaBusinessArchitecture.owl#nextActivity -->

    <ObjectProperty rdf:about="http://www.agilebirds.com/ontologies/CostaBusinessArchitecture.owl#nextActivity">
        <rdfs:range rdf:resource="http://www.agilebirds.com/ontologies/CostaBusinessArchitecture.owl#ValueStreamActivity"/>
        <rdfs:domain rdf:resource="http://www.agilebirds.com/ontologies/CostaBusinessArchitecture.owl#ValueStreamActivity"/>
        <inverseOf rdf:resource="http://www.agilebirds.com/ontologies/CostaBusinessArchitecture.owl#previousActivity"/>
    </ObjectProperty>
    


    <!-- http://www.agilebirds.com/ontologies/CostaBusinessArchitecture.owl#nextObjective -->

    <ObjectProperty rdf:about="http://www.agilebirds.com/ontologies/CostaBusinessArchitecture.owl#nextObjective">
        <rdfs:domain rdf:resource="http://www.agilebirds.com/ontologies/CostaBusinessArchitecture.owl#Goal"/>
        <rdfs:range rdf:resource="http://www.agilebirds.com/ontologies/CostaBusinessArchitecture.owl#Goal"/>
        <rdfs:subPropertyOf rdf:resource="&owl;topObjectProperty"/>
    </ObjectProperty>
    


    <!-- http://www.agilebirds.com/ontologies/CostaBusinessArchitecture.owl#previousActivity -->

    <ObjectProperty rdf:about="http://www.agilebirds.com/ontologies/CostaBusinessArchitecture.owl#previousActivity">
        <rdfs:range rdf:resource="http://www.agilebirds.com/ontologies/CostaBusinessArchitecture.owl#ValueStreamActivity"/>
        <rdfs:domain rdf:resource="http://www.agilebirds.com/ontologies/CostaBusinessArchitecture.owl#ValueStreamActivity"/>
        <rdfs:subPropertyOf rdf:resource="&owl;topObjectProperty"/>
    </ObjectProperty>
    


    <!-- http://www.agilebirds.com/ontologies/CostaBusinessArchitecture.owl#previousObjective -->

    <ObjectProperty rdf:about="http://www.agilebirds.com/ontologies/CostaBusinessArchitecture.owl#previousObjective">
        <rdfs:range rdf:resource="http://www.agilebirds.com/ontologies/CostaBusinessArchitecture.owl#Goal"/>
        <rdfs:domain rdf:resource="http://www.agilebirds.com/ontologies/CostaBusinessArchitecture.owl#Goal"/>
        <inverseOf rdf:resource="http://www.agilebirds.com/ontologies/CostaBusinessArchitecture.owl#nextObjective"/>
    </ObjectProperty>
    


    <!-- 
    ///////////////////////////////////////////////////////////////////////////////////////
    //
    // Data properties
    //
    ///////////////////////////////////////////////////////////////////////////////////////
     -->

    


    <!-- http://www.agilebirds.com/ontologies/CostaBusinessArchitecture.owl#creationDate -->

    <DatatypeProperty rdf:about="http://www.agilebirds.com/ontologies/CostaBusinessArchitecture.owl#creationDate">
        <rdfs:domain rdf:resource="http://www.agilebirds.com/ontologies/CostaBusinessArchitecture.owl#Element"/>
        <rdfs:range rdf:resource="&xsd;string"/>
        <rdfs:subPropertyOf rdf:resource="&owl;topDataProperty"/>
    </DatatypeProperty>
    


    <!-- http://www.agilebirds.com/ontologies/CostaBusinessArchitecture.owl#description -->

    <DatatypeProperty rdf:about="http://www.agilebirds.com/ontologies/CostaBusinessArchitecture.owl#description">
        <rdfs:domain rdf:resource="http://www.agilebirds.com/ontologies/CostaBusinessArchitecture.owl#Element"/>
        <rdfs:range rdf:resource="&xsd;string"/>
    </DatatypeProperty>
    


    <!-- http://www.agilebirds.com/ontologies/CostaBusinessArchitecture.owl#index -->

    <DatatypeProperty rdf:about="http://www.agilebirds.com/ontologies/CostaBusinessArchitecture.owl#index">
        <rdfs:domain rdf:resource="http://www.agilebirds.com/ontologies/CostaBusinessArchitecture.owl#NamedElement"/>
        <rdfs:range rdf:resource="&xsd;int"/>
        <rdfs:subPropertyOf rdf:resource="&owl;topDataProperty"/>
    </DatatypeProperty>
    


    <!-- http://www.agilebirds.com/ontologies/CostaBusinessArchitecture.owl#name -->

    <DatatypeProperty rdf:about="http://www.agilebirds.com/ontologies/CostaBusinessArchitecture.owl#name">
        <rdfs:domain rdf:resource="http://www.agilebirds.com/ontologies/CostaBusinessArchitecture.owl#NamedElement"/>
        <rdfs:range rdf:resource="&xsd;string"/>
    </DatatypeProperty>
    


    <!-- http://www.agilebirds.com/ontologies/CostaBusinessArchitecture.owl#valueStrealReceivingStakeholder -->

    <DatatypeProperty rdf:about="http://www.agilebirds.com/ontologies/CostaBusinessArchitecture.owl#valueStrealReceivingStakeholder">
        <rdfs:domain rdf:resource="http://www.agilebirds.com/ontologies/CostaBusinessArchitecture.owl#ValueStream"/>
        <rdfs:range rdf:resource="&xsd;string"/>
    </DatatypeProperty>
    


    <!-- http://www.agilebirds.com/ontologies/CostaBusinessArchitecture.owl#valueStreamTriggeringStakeholder -->

    <DatatypeProperty rdf:about="http://www.agilebirds.com/ontologies/CostaBusinessArchitecture.owl#valueStreamTriggeringStakeholder">
        <rdfs:domain rdf:resource="http://www.agilebirds.com/ontologies/CostaBusinessArchitecture.owl#ValueStream"/>
        <rdfs:range rdf:resource="&xsd;string"/>
        <rdfs:subPropertyOf rdf:resource="&owl;topDataProperty"/>
    </DatatypeProperty>
    


    <!-- 
    ///////////////////////////////////////////////////////////////////////////////////////
    //
    // Classes
    //
    ///////////////////////////////////////////////////////////////////////////////////////
     -->

    


    <!-- http://www.agilebirds.com/ontologies/CostaBusinessArchitecture.owl#ActivityLink -->

    <Class rdf:about="http://www.agilebirds.com/ontologies/CostaBusinessArchitecture.owl#ActivityLink">
        <rdfs:subClassOf rdf:resource="http://www.agilebirds.com/ontologies/CostaBusinessArchitecture.owl#Association"/>
    </Class>
    


    <!-- http://www.agilebirds.com/ontologies/CostaBusinessArchitecture.owl#Association -->

    <Class rdf:about="http://www.agilebirds.com/ontologies/CostaBusinessArchitecture.owl#Association">
        <rdfs:subClassOf rdf:resource="http://www.agilebirds.com/ontologies/CostaBusinessArchitecture.owl#Classifier"/>
        <rdfs:comment>An association describes a set of tuples whose values refer to typed instances. 
An instance of an association is called a link.</rdfs:comment>
    </Class>
    


    <!-- http://www.agilebirds.com/ontologies/CostaBusinessArchitecture.owl#Capability -->

    <Class rdf:about="http://www.agilebirds.com/ontologies/CostaBusinessArchitecture.owl#Capability">
        <rdfs:subClassOf rdf:resource="http://www.agilebirds.com/ontologies/CostaBusinessArchitecture.owl#CapabilitySystem"/>
        <rdfs:comment>What arze the various capabilitise in your business? Which of them are distinct, necessary or replacable.

Capability is more that competence. There is a difference notheless: a competence is a &quot;human&quot; capability. It&apos;s embodied in a person. You&apos;d be hard put, for instance, to enthrust the competence &quot;provide leadership&quot; to a machine. For now, at least: because a great many competences ha indeed been automated in the past, turning them into capabilities. Historically, for instance, every insurance agent or bank clerk had to be able to calculate the interest on policies and investments. That task has now been taken over by computers - by machines.</rdfs:comment>
    </Class>
    


    <!-- http://www.agilebirds.com/ontologies/CostaBusinessArchitecture.owl#CapabilitySystem -->

    <Class rdf:about="http://www.agilebirds.com/ontologies/CostaBusinessArchitecture.owl#CapabilitySystem">
        <rdfs:subClassOf rdf:resource="http://www.agilebirds.com/ontologies/CostaBusinessArchitecture.owl#EnterpriseSystemElement"/>
        <rdfs:comment>This is the system you use to ensure that the other two enterprise systems are functioning smoothly. Imagine that the restaurant&apos;s oven has broken down; the glasses all need washing; or the chef doesn&apos;t know how to fry a steak properly: if that happenbs, you have a problem. The &quot;capability system&quot; makes sure it doesn&apos;t come to that.</rdfs:comment>
    </Class>
    


    <!-- http://www.agilebirds.com/ontologies/CostaBusinessArchitecture.owl#CapacityContrainer -->

    <Class rdf:about="http://www.agilebirds.com/ontologies/CostaBusinessArchitecture.owl#CapacityContrainer">
        <rdfs:subClassOf rdf:resource="http://www.agilebirds.com/ontologies/CostaBusinessArchitecture.owl#Container"/>
    </Class>
    


    <!-- http://www.agilebirds.com/ontologies/CostaBusinessArchitecture.owl#Classifier -->

    <Class rdf:about="http://www.agilebirds.com/ontologies/CostaBusinessArchitecture.owl#Classifier">
        <rdfs:subClassOf rdf:resource="http://www.agilebirds.com/ontologies/CostaBusinessArchitecture.owl#Type"/>
        <rdfs:comment>A classifier is a classification of instances - it describes a set of instances that have features in common. A classifier can specify a generalization hierarchy by referencing its general classifiers.
A classifier has the capability to own collaboration uses. These collaboration uses link a collaboration with the classifier to give a description of the workings of the classifier.
A classifier has the capability to own use cases. Although the owning classifier typically represents the subject to which the owned use cases apply, this is not necessarily the case. In principle, the same use case can be applied to multiple subjects, as identified by the subject association role of a use case.
Classifier is defined to be a kind of templateable element so that a classifier can be parameterized. It is also defined to be a kind of parameterable element so that a classifier can be a formal template parameter.</rdfs:comment>
    </Class>
    


    <!-- http://www.agilebirds.com/ontologies/CostaBusinessArchitecture.owl#CommitmentSystem -->

    <Class rdf:about="http://www.agilebirds.com/ontologies/CostaBusinessArchitecture.owl#CommitmentSystem">
        <rdfs:label>Commitment</rdfs:label>
        <rdfs:subClassOf rdf:resource="http://www.agilebirds.com/ontologies/CostaBusinessArchitecture.owl#EnterpriseSystemElement"/>
        <rdfs:comment>This maintains contacts and relation swoth the customer. It embraces the services you offer in the form of promises or products. The menu is that tangible manifestion of the commitment system in a restaurant. it sets out all the things the customer can order of what it is you&apos;re promising the customer.</rdfs:comment>
    </Class>
    


    <!-- http://www.agilebirds.com/ontologies/CostaBusinessArchitecture.owl#ConnectableElement -->

    <Class rdf:about="http://www.agilebirds.com/ontologies/CostaBusinessArchitecture.owl#ConnectableElement">
        <rdfs:subClassOf rdf:resource="http://www.agilebirds.com/ontologies/CostaBusinessArchitecture.owl#TypedElement"/>
        <rdfs:comment>ConnectableElement is an abstract metaclass representing a set of instances that play roles of a classifier. Connectable elements may be joined by attached connectors and specify configurations of linked instances to be created within an instance of the containing classifier.
A connectable element may be exposed as a connectable element template parameter.</rdfs:comment>
    </Class>
    


    <!-- http://www.agilebirds.com/ontologies/CostaBusinessArchitecture.owl#Container -->

    <Class rdf:about="http://www.agilebirds.com/ontologies/CostaBusinessArchitecture.owl#Container">
        <rdfs:subClassOf rdf:resource="http://www.agilebirds.com/ontologies/CostaBusinessArchitecture.owl#NamedElement"/>
    </Class>
    


    <!-- http://www.agilebirds.com/ontologies/CostaBusinessArchitecture.owl#CoordinationSystem -->

    <Class rdf:about="http://www.agilebirds.com/ontologies/CostaBusinessArchitecture.owl#CoordinationSystem">
        <rdfs:label>Coordination</rdfs:label>
        <rdfs:subClassOf rdf:resource="http://www.agilebirds.com/ontologies/CostaBusinessArchitecture.owl#OrganisationSystemElement"/>
        <rdfs:comment>This system aligns all the enterprise&apos;s activities with on another: it ensures that resources are handled as efficientyl as possible. All the planning methods you apply in your business form part of the &quot;coordination system&quot;. Work planning supervision and scheduled fall into this category, as does stock management. These things are therefore referred to in the business world as process management, personnel management and resource management.</rdfs:comment>
    </Class>
    


    <!-- http://www.agilebirds.com/ontologies/CostaBusinessArchitecture.owl#CostaElement -->

    <Class rdf:about="http://www.agilebirds.com/ontologies/CostaBusinessArchitecture.owl#CostaElement">
        <rdfs:subClassOf rdf:resource="http://www.agilebirds.com/ontologies/CostaBusinessArchitecture.owl#NamedElement"/>
        <rdfs:comment>NamedElements that belong to Costa  Model and belongs both to a Costa System (Commitment, Delivery, Capability, Coordination, Direction and Risk Control) and an abstractions of the Costa Model ( What, How, Where, When, Who and Why)</rdfs:comment>
    </Class>
    


    <!-- http://www.agilebirds.com/ontologies/CostaBusinessArchitecture.owl#DeliverySystem -->

    <Class rdf:about="http://www.agilebirds.com/ontologies/CostaBusinessArchitecture.owl#DeliverySystem">
        <rdfs:label>Delivery</rdfs:label>
        <rdfs:subClassOf rdf:resource="http://www.agilebirds.com/ontologies/CostaBusinessArchitecture.owl#EnterpriseSystemElement"/>
        <rdfs:comment>Commitments (promises) are obviously  not enough; you also have to keep them. For that reason business also has a &quot;delivery&quot; system. This ensures - to stick with the restaurant metaphor - that the ordered meal eventually ends up on the customer&apos;s plate.</rdfs:comment>
    </Class>
    


    <!-- http://www.agilebirds.com/ontologies/CostaBusinessArchitecture.owl#DirectionSystem -->

    <Class rdf:about="http://www.agilebirds.com/ontologies/CostaBusinessArchitecture.owl#DirectionSystem">
        <rdfs:label>Direction</rdfs:label>
        <rdfs:subClassOf rdf:resource="http://www.agilebirds.com/ontologies/CostaBusinessArchitecture.owl#OrganisationSystemElement"/>
        <rdfs:comment>All the actvities accuring within a business have to fit within its objectives, so a system is also needed to track those objectives and, where necessary, to fine-tune them. In practice, it is wrong to refer here to just one system: there are probably several different direction systems at work within a business. Familiar exemples include budget planning, strategic planning, functinoal and evaluation cycles and performance management. Direction seeks to answer questions like &quot;how do we achieve our goals?&quot; and &quot;what should we be doing differently?&quot;</rdfs:comment>
    </Class>
    


    <!-- http://www.agilebirds.com/ontologies/CostaBusinessArchitecture.owl#Element -->

    <Class rdf:about="http://www.agilebirds.com/ontologies/CostaBusinessArchitecture.owl#Element">
        <rdfs:comment>comment &quot;An element is a constituent of a model. As such, it has the capability of owning other elements.&quot;</rdfs:comment>
    </Class>
    


    <!-- http://www.agilebirds.com/ontologies/CostaBusinessArchitecture.owl#EnterpriseSystemElement -->

    <Class rdf:about="http://www.agilebirds.com/ontologies/CostaBusinessArchitecture.owl#EnterpriseSystemElement">
        <rdfs:label>Enterprise Systems</rdfs:label>
        <rdfs:subClassOf rdf:resource="http://www.agilebirds.com/ontologies/CostaBusinessArchitecture.owl#CostaElement"/>
        <rdfs:comment>Enterprise systems govern the busines&apos;s activity. They ensure that the business can execute in practice what it has undertaken to do. The three systems are: Commitment, Delivery and Capability.</rdfs:comment>
    </Class>
    


    <!-- http://www.agilebirds.com/ontologies/CostaBusinessArchitecture.owl#Goal -->

    <Class rdf:about="http://www.agilebirds.com/ontologies/CostaBusinessArchitecture.owl#Goal">
        <rdfs:label>Objective</rdfs:label>
        <rdfs:subClassOf rdf:resource="http://www.agilebirds.com/ontologies/CostaBusinessArchitecture.owl#DirectionSystem"/>
    </Class>
    


    <!-- http://www.agilebirds.com/ontologies/CostaBusinessArchitecture.owl#HotMapValue -->

    <Class rdf:about="http://www.agilebirds.com/ontologies/CostaBusinessArchitecture.owl#HotMapValue">
        <rdfs:subClassOf rdf:resource="http://www.agilebirds.com/ontologies/CostaBusinessArchitecture.owl#Value"/>
    </Class>
    


    <!-- http://www.agilebirds.com/ontologies/CostaBusinessArchitecture.owl#NamedElement -->

    <Class rdf:about="http://www.agilebirds.com/ontologies/CostaBusinessArchitecture.owl#NamedElement">
        <rdfs:subClassOf rdf:resource="http://www.agilebirds.com/ontologies/CostaBusinessArchitecture.owl#Element"/>
        <rdfs:comment>A named element is an element in a model that may have a name.
A named element supports using a string expression to specify its name. This allows names of model elements to involve template parameters. The actual name is evaluated from the string expression only when it is sensible to do so (e.g., when a template is bound).</rdfs:comment>
    </Class>
    


    <!-- http://www.agilebirds.com/ontologies/CostaBusinessArchitecture.owl#ObjectiveLink -->

    <Class rdf:about="http://www.agilebirds.com/ontologies/CostaBusinessArchitecture.owl#ObjectiveLink">
        <rdfs:subClassOf rdf:resource="http://www.agilebirds.com/ontologies/CostaBusinessArchitecture.owl#Association"/>
    </Class>
    


    <!-- http://www.agilebirds.com/ontologies/CostaBusinessArchitecture.owl#OpenFlexoTypes -->

    <Class rdf:about="http://www.agilebirds.com/ontologies/CostaBusinessArchitecture.owl#OpenFlexoTypes"/>
    


    <!-- http://www.agilebirds.com/ontologies/CostaBusinessArchitecture.owl#OrganisationSystemElement -->

    <Class rdf:about="http://www.agilebirds.com/ontologies/CostaBusinessArchitecture.owl#OrganisationSystemElement">
        <rdfs:label>Organisation Systems</rdfs:label>
        <rdfs:subClassOf rdf:resource="http://www.agilebirds.com/ontologies/CostaBusinessArchitecture.owl#CostaElement"/>
    </Class>
    


    <!-- http://www.agilebirds.com/ontologies/CostaBusinessArchitecture.owl#ProductSegmentation -->

    <Class rdf:about="http://www.agilebirds.com/ontologies/CostaBusinessArchitecture.owl#ProductSegmentation">
        <rdfs:label>Value Proposition</rdfs:label>
        <rdfs:subClassOf rdf:resource="http://www.agilebirds.com/ontologies/CostaBusinessArchitecture.owl#CommitmentSystem"/>
        <rdfs:comment>What de we promise our customers? In what form do we make those promises? How do we manage these promises? What are the different &quot;groups&quot; of products we use and what promises do they meet?</rdfs:comment>
    </Class>
    


    <!-- http://www.agilebirds.com/ontologies/CostaBusinessArchitecture.owl#ProductSegmentationContainer -->

    <Class rdf:about="http://www.agilebirds.com/ontologies/CostaBusinessArchitecture.owl#ProductSegmentationContainer">
        <rdfs:subClassOf rdf:resource="http://www.agilebirds.com/ontologies/CostaBusinessArchitecture.owl#Container"/>
    </Class>
    


    <!-- http://www.agilebirds.com/ontologies/CostaBusinessArchitecture.owl#Property -->

    <Class rdf:about="http://www.agilebirds.com/ontologies/CostaBusinessArchitecture.owl#Property">
        <rdfs:subClassOf rdf:resource="http://www.agilebirds.com/ontologies/CostaBusinessArchitecture.owl#ConnectableElement"/>
        <rdfs:comment>A property is a structural feature of a classifier that characterizes instances of the classifier. 

A property related by ownedAttribute to a classifier (other than an association) represents an attribute and might also represent an association end. It relates an instance of the class to a value or set of values of the type of the attribute. A property related by memberEnd or its specializations to an association represents an end of the association. The type of the property is the type of the end of the association.

A property represents a set of instances that are owned by a containing classifier instance.

A property has the capability of being a deployment target in a deployment relationship. This enables modeling the deployment to hierarchical nodes that have properties functioning as internal parts.

Property represents a declared state of one or more instances in terms of a named relationship to a value or values. When a property is an attribute of a classifier, the value or values are related to the instance of the classifier by being held in slots of the instance. When a property is an association end, the value or values are related to the instance or instances at the other end(s) of the association. 

The range of valid values represented by the property can be controlled by setting the property&apos;s type.
Property specializes ParameterableElement to specify that a property can be exposed as a formal template parameter, and provided as an actual parameter in a binding of a template.</rdfs:comment>
    </Class>
    


    <!-- http://www.agilebirds.com/ontologies/CostaBusinessArchitecture.owl#RiskControlSystem -->

    <Class rdf:about="http://www.agilebirds.com/ontologies/CostaBusinessArchitecture.owl#RiskControlSystem">
        <rdfs:label>Risk Control</rdfs:label>
        <rdfs:subClassOf rdf:resource="http://www.agilebirds.com/ontologies/CostaBusinessArchitecture.owl#OrganisationSystemElement"/>
        <rdfs:comment>The risk contraol system also consists of various &quot;sub-systems&quot; that may or may not have been installed. Some of them are permanent and internal, while others are time-limited and external. Audits, for instance, are often performed by an external partner, while bookkeeping is mostly done internally. The objective of both systems is to mitigate the risks to which the business is exposed.

Lots more risk systems can obviously be imagined: quality control, say, or environmental protection. These ensure that you are not running any risks with respect to customers and the outside world.</rdfs:comment>
    </Class>
    


    <!-- http://www.agilebirds.com/ontologies/CostaBusinessArchitecture.owl#ServiceBreakdown -->

    <Class rdf:about="http://www.agilebirds.com/ontologies/CostaBusinessArchitecture.owl#ServiceBreakdown">
        <rdfs:label>Service Breakdown</rdfs:label>
        <rdfs:subClassOf rdf:resource="http://www.agilebirds.com/ontologies/CostaBusinessArchitecture.owl#DeliverySystem"/>
        <rdfs:comment>How do you tranlsate a customer&apos;s request into a (limited) number of activities or processes that you run through in your business to bring about what the curtomer asked for ?</rdfs:comment>
    </Class>
    


    <!-- http://www.agilebirds.com/ontologies/CostaBusinessArchitecture.owl#ServiceBreakdownContainer -->

    <Class rdf:about="http://www.agilebirds.com/ontologies/CostaBusinessArchitecture.owl#ServiceBreakdownContainer">
        <rdfs:subClassOf rdf:resource="http://www.agilebirds.com/ontologies/CostaBusinessArchitecture.owl#Container"/>
    </Class>
    


    <!-- http://www.agilebirds.com/ontologies/CostaBusinessArchitecture.owl#Type -->

    <Class rdf:about="http://www.agilebirds.com/ontologies/CostaBusinessArchitecture.owl#Type">
        <rdfs:subClassOf rdf:resource="http://www.agilebirds.com/ontologies/CostaBusinessArchitecture.owl#NamedElement"/>
        <rdfs:comment>
An optional association that specifies the link corresponding to this connector.

&quot;A type is a named element that is used as the type for a typed element. 
A type constrains the values represented by a typed element.&quot;</rdfs:comment>
        <rdfs:comment>This information is derived from the return result for this Operation.
The type of the TypedElement.</rdfs:comment>
    </Class>
    


    <!-- http://www.agilebirds.com/ontologies/CostaBusinessArchitecture.owl#TypedElement -->

    <Class rdf:about="http://www.agilebirds.com/ontologies/CostaBusinessArchitecture.owl#TypedElement">
        <rdfs:subClassOf rdf:resource="http://www.agilebirds.com/ontologies/CostaBusinessArchitecture.owl#NamedElement"/>
        <rdfs:comment>A typed element is a kind of named element that represents an element with a type.
A typed element has a type.</rdfs:comment>
    </Class>
    


    <!-- http://www.agilebirds.com/ontologies/CostaBusinessArchitecture.owl#Value -->

    <Class rdf:about="http://www.agilebirds.com/ontologies/CostaBusinessArchitecture.owl#Value">
        <rdfs:subClassOf rdf:resource="http://www.agilebirds.com/ontologies/CostaBusinessArchitecture.owl#Element"/>
    </Class>
    


    <!-- http://www.agilebirds.com/ontologies/CostaBusinessArchitecture.owl#ValueStream -->

    <Class rdf:about="http://www.agilebirds.com/ontologies/CostaBusinessArchitecture.owl#ValueStream">
        <rdfs:label>Value Stream</rdfs:label>
        <rdfs:subClassOf rdf:resource="http://www.agilebirds.com/ontologies/CostaBusinessArchitecture.owl#Container"/>
        <rdfs:subClassOf rdf:resource="http://www.agilebirds.com/ontologies/CostaBusinessArchitecture.owl#CoordinationSystem"/>
    </Class>
    


    <!-- http://www.agilebirds.com/ontologies/CostaBusinessArchitecture.owl#ValueStreamActivity -->

    <Class rdf:about="http://www.agilebirds.com/ontologies/CostaBusinessArchitecture.owl#ValueStreamActivity">
        <rdfs:label>Activity</rdfs:label>
        <rdfs:subClassOf rdf:resource="http://www.agilebirds.com/ontologies/CostaBusinessArchitecture.owl#CoordinationSystem"/>
    </Class>
    


    <!-- http://www.agilebirds.com/ontologies/CostaBusinessArchitecture.owl#View -->

    <Class rdf:about="http://www.agilebirds.com/ontologies/CostaBusinessArchitecture.owl#View">
        <rdfs:subClassOf rdf:resource="http://www.agilebirds.com/ontologies/CostaBusinessArchitecture.owl#OpenFlexoTypes"/>
    </Class>
    


    <!-- 
    ///////////////////////////////////////////////////////////////////////////////////////
    //
    // Individuals
    //
    ///////////////////////////////////////////////////////////////////////////////////////
     -->

    


    <!-- http://www.agilebirds.com/ontologies/CostaBusinessArchitecture.owl#Green -->

    <NamedIndividual rdf:about="http://www.agilebirds.com/ontologies/CostaBusinessArchitecture.owl#Green">
        <rdf:type rdf:resource="http://www.agilebirds.com/ontologies/CostaBusinessArchitecture.owl#HotMapValue"/>
    </NamedIndividual>
    


    <!-- http://www.agilebirds.com/ontologies/CostaBusinessArchitecture.owl#Orange -->

    <NamedIndividual rdf:about="http://www.agilebirds.com/ontologies/CostaBusinessArchitecture.owl#Orange">
        <rdf:type rdf:resource="http://www.agilebirds.com/ontologies/CostaBusinessArchitecture.owl#HotMapValue"/>
    </NamedIndividual>
    


    <!-- http://www.agilebirds.com/ontologies/CostaBusinessArchitecture.owl#Red -->

    <NamedIndividual rdf:about="http://www.agilebirds.com/ontologies/CostaBusinessArchitecture.owl#Red">
        <rdf:type rdf:resource="http://www.agilebirds.com/ontologies/CostaBusinessArchitecture.owl#HotMapValue"/>
    </NamedIndividual>
</rdf:RDF>



<!-- Generated by the OWL API (version 3.4.2) http://owlapi.sourceforge.net -->

